optional backend compilation

coqjit/flags.ml
@@ -2,5 +2,6 @@ let debug_stk = ref false
 let safe_mode = ref false
 let print_asm_end = ref false
 let print_chkpts = ref false
-let allow_opt = ref true
+let allow_compile = ref true
 let allow_spec = ref true
+let allow_opts = ref true
